src/case_study/list_example.v
@@ -1,0 +1,178 @@
+From iris.base_logic Require Export gen_heap.
+From iris.algebra Require Export list excl_auth.
+From nextgen.case_study.program_logic Require Import CC_ectx_lifting
+     CC_ectxi_language CC_ectx_lifting weakestpre.
+From nextgen.case_study Require Export stack_lang stack_transform.
+From iris.proofmode Require Import tactics.
+From stdpp Require Import fin_maps.
+
+From nextgen Require Import nextgen_independent.
+From nextgen.lib Require Import invariants.
+From nextgen.case_study Require Import rules_unary stack_lang_notation.
+
+Set Default Proof Using "Type".
+Import uPred.
+
+Lemma fill_inner_cons n e K Ks :
+  fill (K :: Ks) (n,e) = fill Ks (n, fill_item K e).
+Proof. auto. Qed.
+Lemma fill_to_CC_fill K n e :
+  CC_ectxi_language.fill K (n,e) = fill K (n,e).
+Proof. auto. Qed.
+
+Ltac peel_ctx :=
+  try rewrite fill_to_CC_fill; rewrite fill_inner_cons; simpl fill_item.
+
+Ltac prepare_ctx :=
+  (try rewrite /stack_fill_item /=) ;
+  let H := fresh "H" in
+  match goal with
+  | |- context [ WP (?n,?e) @ _ ; ↑ _ ; _ {{ _ }}%I ] =>
+      pose proof (construct_ctx_eq n e) as H;try rewrite /= to_of_val in H;
+      try (rewrite H; clear H; simpl app); peel_ctx
+      end.
+
+Section list_code.
+  Open Scope val_scope.
+
+  Definition heap_cons : val :=
+    λ: global, <>, "x" "xs" := let: "p" := ⟪"x","xs"⟫ in
+                               SOME (href "p").
+
+  Definition heap_map_list : val :=
+    rec: global, <>, "map_list", "f" "l" :=
+      match: "l" with
+        NONE => NONE
+      | SOME "p" =>
+          let: "hd" := Fst !"p" in
+          let: "tl" := Snd !"p" in
+          heap_cons ("f" "hd") ("map_list" "tl")
+      end.
+
+  Definition stack_cons : val :=
+    λ: global, <>, "x" "xs" := let: "p" := ⟪"x","xs"⟫ in
+                               SOME (sref "p").
+
+  Definition stack_map_list : val :=
+    rec: global, <>, "map_list", "f" "l" :=
+      match: "l" with
+        NONE => NONE
+      | SOME "p" =>
+          let: "hd" := Fst !"p" in
+          let: "tl" := Snd !"p" in
+          stack_cons ("f" "hd") ("map_list" "tl")
+      end.
+
+  Definition empty_list : val := NONEV.
+      
+End list_code.
+
+Section list_prec.
+  Context `{!heapGS Σ Ω}.
+
+  Fixpoint is_heap_list_nat (hd : val) (xs : list nat) : iProp Σ :=
+    match xs with
+    | [] => ⌜hd = NONEV⌝
+    | x :: xs => ∃ l hd', ⌜hd = SOMEV #(global,l)⌝ ∗ l ↦ ⟪x,hd'⟫ ∗ is_heap_list_nat hd' xs
+  end%I.
+
+  Fixpoint is_stack_list_nat (i : nat) (hd : val) (xs : list nat) : iProp Σ :=
+    match xs with
+    | [] => ⌜hd = NONEV⌝
+    | x :: xs => ∃ l hd' j, ⌜hd = SOMEV #(global,l)⌝ ∗ ⌜j <= i⌝ ∗ j @@ l ↦ ⟪x,hd'⟫ ∗ is_stack_list_nat i hd' xs
+  end%I.
+
+  Lemma is_heap_list_nat_intro hd xs lft :
+    is_heap_list_nat hd xs ⊢ ⚡={Ω <- lft}=> is_heap_list_nat hd xs.
+  Proof.
+    revert hd. induction xs=>hd.
+    - simpl. iIntros "%". iModIntro. auto.
+    - simpl.
+      iIntros "(%l & %hd' & %Heq & Hl & Hlist)".
+      iDestruct (IHxs with "Hlist") as "Hlist".
+      iModIntro. iExists _,_. iFrame. auto.
+  Qed.
+
+  Lemma is_heap_list_shift hd xs :
+    is_heap_list_nat hd xs -∗ ⌜∀ n, shift_val hd n = Some hd⌝.
+  Proof.
+    iIntros "Hlist" (n).
+    destruct xs.
+    - simpl. iDestruct "Hlist" as %->. simpl. auto.
+    - simpl. iDestruct "Hlist" as "(%l & %hd' & -> & Hl & Hlist)".
+      simpl. auto.
+  Qed.
+
+  Lemma is_heap_list_permanent hd xs :
+    is_heap_list_nat hd xs -∗ ⌜permanent hd⌝.
+  Proof.
+    iIntros "Hlist".
+    destruct xs.
+    - simpl. iDestruct "Hlist" as %->. iPureIntro. repeat constructor.
+    - simpl. iDestruct "Hlist" as "(%l & %hd' & -> & Hl & Hlist)".
+      iPureIntro. repeat constructor.
+  Qed.
+
+  Lemma is_stack_list_nat_intro i hd xs j :
+    i < j ->
+    is_stack_list_nat i hd xs ⊢ ⚡={Ω <- ^j}=> is_stack_list_nat i hd xs.
+  Proof.
+    intros Hlt.
+    revert hd. induction xs=>hd.
+    - simpl. iIntros "%". iModIntro. auto.
+    - simpl.
+      iIntros "(%l & %hd' & %i' & %Heq & %Hle & Hl & Hlist)".
+      iDestruct (IHxs with "Hlist") as "Hlist".
+      iDestruct (stack_stack_pop_intro _ _ _ _ j with "Hl") as "Hl";[lia|].
+      iModIntro. iExists _,_,_. iFrame. auto.
+  Qed.
+
+  Lemma is_stack_list_nat_weaken i i' hd xs :
+    i <= i' ->
+    is_stack_list_nat i hd xs ⊢ is_stack_list_nat i' hd xs.
+  Proof.
+    revert hd. induction xs=>hd.
+    - simpl. auto.
+    - simpl.
+      iIntros (Hle) "(%l & %hd' & %j & %Heq & %Hj & Hl & Hlist)".
+      iDestruct (IHxs with "Hlist") as "Hlist";auto.
+      iExists _,_,_. iFrame. iSplit;auto.
+      iPureIntro. lia.
+  Qed.
+
+  #[global] Instance is_heap_list_nat_intro' hd xs lft
+    : IntoPnextgen _ _ _ := is_heap_list_nat_intro hd xs lft.
+  
+End list_prec.
+
+Section list_spec.
+  Context `{!heapGS Σ Ω}.
+  
+  Lemma heap_list_cons_spec hd xs (n : nat) m :
+    {{{ [size] m ∗ is_heap_list_nat hd xs }}}
+      (m,heap_cons n hd) @ ↑^m
+    {{{ hd', RET hd'; [size] m ∗ is_heap_list_nat hd'.2 (n :: xs) }}}.
+  Proof.
+    iIntros (Φ) "[Hsize Hlist] #HΦ /=". prepare_ctx.
+    iApply wp_call_global;[eauto|iFrame]. iIntros "!> Hsize /=". prepare_ctx.
+    iApply wp_return;[replace (S m - 1) with m by lia;apply rc_l|auto|lia|iFrame].
+    iIntros "!> Hsize /=". replace (m - 0) with m by lia. iModIntro. rewrite /stack_fill_item /=.
+    eassert (fill [] _ = _) as <-;eauto.
+    iDestruct (is_heap_list_shift with "Hlist") as %Hshift.
+    iApply wp_call_global;[eauto|eauto|iFrame]. iIntros "!> Hsize /=". prepare_ctx.
+    iApply wp_LetIn;[|iIntros "!> /=";simpl subst'].
+    { instantiate (1:=(_,⟪#nv n,_⟫%V)). rewrite /IntoVal/=/stack_of_val. f_equal;eauto. }
+    prepare_ctx. iDestruct (is_heap_list_permanent with "Hlist") as %Hpermanent.
+    iApply wp_heap_alloc.
+    { instantiate (1:=⟪#nv n,_⟫%V). rewrite /IntoVal/=/stack_of_val. f_equal;eauto. }
+    { constructor;auto. constructor. }
+    iIntros "!> %l Hl /=". prepare_ctx.
+    iApply wp_return;[replace (S m - 1) with m by lia;apply rc_l|auto|lia|iFrame].
+    iIntros "!> Hsize". iModIntro. simpl. replace (m - 0) with m by lia.
+    iApply wp_value. simpl.
+    iApply "HΦ". iFrame. iExists l,hd.
+    simpl. iFrame. auto.
+  Qed.
+
+    
+End list_spec.
